Start adapting tree semantics proof to Linden group maps

WarblreEquiv/LWEquivTree.v
@@ -1,6 +1,7 @@
 From Linden Require Import TMatching Tree Chars Semantics MSInput
-  Regex LindenParameters RegexpTranslation ListLemmas
-  WarblreLemmas Tactics LWEquivTreeLemmas LWEquivTMatcher LWEquivTMatcherLemmas NumericLemmas LKFactorization CharDescrCharSet CharSet.
+  Regex LindenParameters RegexpTranslation ListLemmas Groups
+  WarblreLemmas Tactics LWEquivTreeLemmas LWEquivTMatcher LWEquivTMatcherLemmas
+  NumericLemmas LKFactorization CharDescrCharSet CharSet GroupMapMS.
 From Warblre Require Import Result Notation RegExpRecord Match Base
   Patterns Node NodeProps Semantics.
 From Coq Require Import List ZArith Lia.
@@ -22,84 +23,96 @@ Section LWEquivTree.
 
   (** ** Definition of the validity of tree matchers and tree matcher continuations *)
 
-  (* `tMC_is_tree tmc rer cont inp dir` means that the TMatcherContinuation tmc, when run with a MatchState
-    compatible with input inp and valid with respect to rer, performs the actions in the continuation cont and yields a valid priority tree wrt direction dir. *)
-  Definition tMC_is_tree (tmc: TMatcherContinuation) (rer: RegExpRecord) (cont: continuation) (inp: input) (dir: Direction) :=
-    forall (ms: MatchState) (t: tree),
+  (* `tMC_is_tree tmc gl rer actions inp dir` means that the TMatcherContinuation tmc
+    closes the groups defined in gl and, when run with a MatchState
+    compatible with input inp and valid with respect to rer, performs the actions in the
+    list actions and yields a valid priority tree wrt direction dir and the group map
+    corresponding to the MatchState and the list of open groups. *)
+  Definition tMC_is_tree (tmc: TMatcherContinuation) (gl: open_groups) (rer: RegExpRecord) (actions: actions) (inp: input) (dir: Direction) :=
+    forall (ms: MatchState) (gm: GroupMap.t) (t: tree),
       ms_matches_inp ms inp ->
       tmc ms = Success t ->
-      is_tree Epsilon cont inp dir t.
+      equiv_groupmap_ms gm ms ->
+      group_map_equiv_open_groups gm gl ->
+      is_tree actions inp gm dir t.
 
-  (* `tMC_valid tmc rer cont str0 dir` means that the TMatcherContinuation tmc, when run on any input compatible with the string str0 under the flags in rer,
-     performs the actions in the continuation cont and yields a valid priority tree wrt direction dir. *)
-  Definition tMC_valid (tmc: TMatcherContinuation) (rer: RegExpRecord) (cont: continuation) (str0: string) (dir: Direction) :=
-    forall inp, input_compat inp str0 -> tMC_is_tree tmc rer cont inp dir.
+  (* `tMC_valid tmc gl rer actions str0 dir` means that the TMatcherContinuation tmc closes
+    the groups defined in gl and, when run on any input compatible with the string str0 under
+    the flags in rer, performs the actions in the list actions and yields a valid priority
+    tree wrt direction dir. *)
+  Definition tMC_valid (tmc: TMatcherContinuation) (gl: open_groups) (rer: RegExpRecord) (actions: actions) (str0: string) (dir: Direction) :=
+    forall inp, input_compat inp str0 -> tMC_is_tree tmc gl rer actions inp dir.
 
   (* `tm_valid tm rer lreg dir` means that under the given RegExpRecord (set of flags), the TMatcher tm recognizes the regexp lreg with direction dir on any input, and yields a valid priority tree. *)
   Definition tm_valid (tm: TMatcher) (rer: RegExpRecord) (lreg: regex) (dir: Direction) :=
-    forall (tmc: TMatcherContinuation) (cont: continuation) (str0: string),
-    tMC_valid tmc rer cont str0 dir ->
-    tMC_valid (fun s => tm s tmc) rer (Areg lreg::cont) str0 dir.
+    forall (tmc: TMatcherContinuation) (gl: open_groups) (actions: actions) (str0: string),
+    open_groups_disjoint gl (def_groups lreg) ->
+    tMC_valid tmc gl rer actions str0 dir ->
+    tMC_valid (fun s => tm s tmc) gl rer (Areg lreg::actions) str0 dir.
 
 
-  (* Validity of empty continuation *)
+  (* Validity of empty continuation, which does not close any group and does not perform any action *)
   Lemma id_tmcont_valid:
-    forall rer str dir, tMC_valid id_tmcont rer [] str dir.
+    forall rer str dir, tMC_valid id_tmcont [] rer [] str dir.
   Proof.
-    intros rer str dir inp Hinp_compat ms t Hmsinp Heqt.
+    intros rer str dir inp Hinp_compat ms gm t Hmsinp Heqt Hgmms Hgmgl.
     injection Heqt as <-. apply tree_epsilon.
   Qed.
 
 
   (** ** Lemmas for repeated matching: *)
   (* Lemma for the case where the min is nonzero *)
-  Lemma tRepeatMatcher'_minnonzero_valid:
+  Lemma tRepeatMatcher'_forced_valid:
     (* For all repeat matcher parameters (except min), *)
-    forall rer greedy parenIndex parenCount plus,
+    forall rer greedy parenIndex parenCount delta,
     forall (tm: TMatcher) (lreg: regex) (dir: Direction),
       (* if the TMatcher tm is valid wrt lreg and direction dir, *)
       tm_valid tm rer lreg dir ->
       (* the list of capture groups of lreg matches the repeat matcher parameters, *)
       def_groups lreg = List.seq (parenIndex + 1) parenCount ->
-      (* and the repeat matcher with min=0 is valid wrt Quantified greedy 0 plus lreg and direction dir, *)
-      (forall fuel, tm_valid (fun s tmc => tRepeatMatcher' tm dir 0 plus greedy s tmc parenIndex parenCount fuel) rer (Regex.Quantified greedy 0 plus lreg) dir) ->
-      (* then all repeat matchers with any min are valid wrt Quantified greedy min plus lreg and direction dir. *)
-      forall mini fuel, tm_valid (fun s tmc => tRepeatMatcher' tm dir mini (NoI.N mini + plus)%NoI greedy s tmc parenIndex parenCount fuel) rer (Regex.Quantified greedy mini plus lreg) dir.
+      (* and the repeat matcher with min=0 is valid wrt Quantified greedy 0 delta lreg and direction dir, *)
+      (forall fuel, tm_valid (fun s tmc => tRepeatMatcher' tm dir 0 delta greedy s tmc parenIndex parenCount fuel) rer (Regex.Quantified greedy 0 delta lreg) dir) ->
+      (* then all repeat matchers with any min are valid wrt Quantified greedy min delta lreg and direction dir. *)
+      forall mini fuel, tm_valid (fun s tmc => tRepeatMatcher' tm dir mini (NoI.N mini + delta)%NoI greedy s tmc parenIndex parenCount fuel) rer (Regex.Quantified greedy mini delta lreg) dir.
   Proof.
-    intros rer greedy parenIndex parenCount plus tm lreg dir Htm_valid Hgroups_valid Hminzero_valid.
+    intros rer greedy parenIndex parenCount delta tm lreg dir Htm_valid Hgroups_valid Hminzero_valid.
     intro mini. induction mini as [|mini' IHmini'].
-    1: { simpl. replace (match plus with | NoI.N r' => _ | +∞ => _ end) with plus by now destruct plus. apply Hminzero_valid. }
+    1: { simpl. replace (match delta with | NoI.N r' => _ | +∞ => _ end) with delta by now destruct delta. apply Hminzero_valid. }
 
     intros [|fuel].
-    1: { simpl. now constructor. }
-    unfold tm_valid. intros tmc cont str0 Htmc_valid. unfold tMC_valid. intros inp Hinp_compat. unfold tMC_is_tree. intros ms t Hmsinp.
+    1: { simpl. unfold tm_valid. intros. unfold tMC_valid. intros. unfold tMC_is_tree. discriminate. }
+    unfold tm_valid. intros tmc gl actions str0 Hgldisj Htmc_valid. unfold tMC_valid. intros inp Hinp_compat. unfold tMC_is_tree. intros ms gm t Hmsinp.
     simpl.
-    replace (match plus with | NoI.N r' => _ | +∞ => _ end =? NoI.N (nat_to_nni 0))%NoI with false by now destruct plus.
+    replace (match delta with | NoI.N r' => _ | +∞ => _ end =? NoI.N (nat_to_nni 0))%NoI with false by now destruct delta.
     destruct List.List.Update.Nat.Batch.update as [cap'|] eqn:Hcapsucc; simpl. 2: discriminate.
     replace (mini' - 0) with mini' by lia.
-    pose proof mini_plus_plusminus_one mini' plus as Hplusminusone. simpl in Hplusminusone. rewrite Hplusminusone. clear Hplusminusone.
-    set (nextplus := match plus with | NoI.N r' => _ | +∞ => _ end).
+    pose proof mini_plus_plusminus_one mini' delta as Hplusminusone. simpl in Hplusminusone. rewrite Hplusminusone by reflexivity. (* ??? *) clear Hplusminusone.
+    set (nextdelta := match delta with | NoI.N r' => _ | +∞ => _ end).
     set (tmcnext := fun y => _).
-    unfold tm_valid in Htm_valid. specialize (Htm_valid tmcnext (Areg (Regex.Quantified greedy mini' plus lreg)::cont) str0).
+    unfold tm_valid in Htm_valid. specialize (Htm_valid tmcnext gl (Areg (Regex.Quantified greedy mini' delta lreg)::actions) str0).
+    specialize_prove Htm_valid by admit. (* Disjointness from quantifier implies disjointness from sub-regexp *)
     specialize_prove Htm_valid. {
-      specialize (IHmini' fuel tmc cont str0 Htmc_valid). simpl in IHmini'. (* Morally, apply IHmini', but there is a monad rewrite under a lambda which we cannot do... *)
+      specialize (IHmini' fuel tmc gl actions str0 Hgldisj Htmc_valid). simpl in IHmini'. (* Morally, apply IHmini', but there is a monad rewrite under a lambda which we cannot do... *)
       unfold tMC_valid, tMC_is_tree. intros inp' Hinp'compat ms' t' Hms'inp.
       unfold tmcnext. rewrite (@monad_id _ _ Errors.match_assertion_error). now apply IHmini'.
     }
     unfold tMC_valid in Htm_valid. specialize (Htm_valid inp Hinp_compat).
     set (msreset := match_state _ _ cap'). unfold tMC_is_tree in Htm_valid.
-    specialize (Htm_valid msreset).
+    specialize (Htm_valid msreset (GroupMap.reset (seq (parenIndex+1) parenCount) gm)).
     destruct tm as [subtree|]; simpl. 2: discriminate.
-    specialize (Htm_valid subtree). 2: reflexivity. (* ??? *)
+    specialize (Htm_valid subtree).
     specialize_prove Htm_valid. { apply ms_matches_inp_capchg with (cap := MatchState.captures ms). now destruct ms. }
     specialize (Htm_valid eq_refl).
-    intro Heqt. injection Heqt as <-.
-    apply tree_pop_reg. apply tree_quant_minpos. 1: congruence. now inversion Htm_valid.
-  Qed.
+    specialize_prove Htm_valid by admit.
+    specialize_prove Htm_valid by admit.
+
+    intro Heqt. injection Heqt as <-. intros Hgmms Hgmgl.
+    apply tree_quant_forced. 1: congruence. assumption.
+  Admitted.
 
 
   (* Lemma for the case where both the min and the max are zero *)
-  Lemma tRepeatMatcher'_zero_valid:
+  Lemma tRepeatMatcher'_done_valid:
     forall rer greedy parenIndex parenCount,
     forall (tm: TMatcher) (lreg: regex) (dir: Direction),
       tm_valid tm rer lreg dir ->
@@ -114,26 +127,26 @@ Section LWEquivTree.
 
 
   (* Lemma for the case where the min is zero but the max is arbitrary *)
-  Lemma tRepeatMatcher'_minzero_valid:
+  Lemma tRepeatMatcher'_free_valid:
     forall rer greedy parenIndex parenCount,
     forall (tm: TMatcher) (lreg: regex) (dir: Direction),
       tm_valid tm rer lreg dir ->
       def_groups lreg = List.seq (parenIndex + 1) parenCount ->
-      forall fuel plus, tm_valid (fun s tmc => tRepeatMatcher' tm dir 0 plus greedy s tmc parenIndex parenCount fuel) rer (Regex.Quantified greedy 0 plus lreg) dir.
+      forall fuel delta, tm_valid (fun s tmc => tRepeatMatcher' tm dir 0 delta greedy s tmc parenIndex parenCount fuel) rer (Regex.Quantified greedy 0 delta lreg) dir.
   Proof.
     intros rer greedy parenIndex parenCount tm lreg dir Htmvalid Hgroupsvalid fuel.
     induction fuel as [|fuel IHfuel].
     1: discriminate.
 
-    intro plus.
-    destruct (plus =? NoI.N (nat_to_nni 0))%NoI eqn:Hpluszero.
-    1: { rewrite noi_eqb_eq in Hpluszero. subst plus. now apply tRepeatMatcher'_zero_valid. }
+    intro delta.
+    destruct (delta =? NoI.N (nat_to_nni 0))%NoI eqn:Hpluszero.
+    1: { rewrite noi_eqb_eq in Hpluszero. subst delta. now apply tRepeatMatcher'_zero_valid. }
     simpl. rewrite Hpluszero.
     intros tmc cont str0 Htmc_valid inp Hinp_compat ms t Hms_inp HmatchSuccess.
     destruct List.List.Update.Nat.Batch.update as [cap'|] eqn:Heqcap'; simpl in *. 2: discriminate.
     set (tmcloop := fun y: MatchState => if (_ =? _)%Z then _ else _) in HmatchSuccess.
     set (msreset := match_state _ _ cap') in HmatchSuccess.
-    assert (tMC_valid tmcloop rer (Acheck (ms_suffix ms dir)::Areg (Regex.Quantified greedy 0 (plus - 1)%NoI lreg)::cont) str0 dir) as Htmcloop_valid. {
+    assert (tMC_valid tmcloop rer (Acheck (ms_suffix ms dir)::Areg (Regex.Quantified greedy 0 (delta - 1)%NoI lreg)::cont) str0 dir) as Htmcloop_valid. {
       intros inp' Hinp'_compat ms1 t1 Hms1_inp Htmcloop_succeeds.
       unfold tmcloop in Htmcloop_succeeds.
       destruct (_ =? _)%Z eqn:Heqcheck.
@@ -154,9 +167,9 @@ Section LWEquivTree.
         injection Htmcloop_succeeds as <-.
         apply tree_pop_check.
         + eapply endInd_neq_advanced; eauto.
-        + rewrite noi_decr in Heqsubtree. specialize (IHfuel (plus - 1)%NoI tmc cont str0 Htmc_valid inp' Hinp'_compat ms1 subtree Hms1_inp Heqsubtree). apply IHfuel.
+        + rewrite noi_decr in Heqsubtree. specialize (IHfuel (delta - 1)%NoI tmc cont str0 Htmc_valid inp' Hinp'_compat ms1 subtree Hms1_inp Heqsubtree). apply IHfuel.
     }
-    specialize (Htmvalid tmcloop (Acheck (ms_suffix ms dir)::Areg (Regex.Quantified greedy 0 (plus-1)%NoI lreg)::cont) str0 Htmcloop_valid inp Hinp_compat).
+    specialize (Htmvalid tmcloop (Acheck (ms_suffix ms dir)::Areg (Regex.Quantified greedy 0 (delta-1)%NoI lreg)::cont) str0 Htmcloop_valid inp Hinp_compat).
     specialize (Htmc_valid inp Hinp_compat).
     unfold tMC_is_tree in Htmvalid, Htmc_valid.
     assert (ms_matches_inp msreset inp) as Hmsreset_inp. {
@@ -170,7 +183,7 @@ Section LWEquivTree.
       specialize (Htmvalid msreset z Hmsreset_inp Heqz).
       specialize (Htmc_valid ms z' Hms_inp Heqz').
       apply tree_pop_reg.
-      rewrite noi_nonzero_succprec with (x := plus). 2: now apply noi_eqb_neq.
+      rewrite noi_nonzero_succprec with (x := delta). 2: now apply noi_eqb_neq.
       eapply tree_quant_minzero_pluspos.
       * symmetry. apply Hgroupsvalid.
       * rewrite ms_suffix_current_str with (ms := ms). 2: assumption.
@@ -185,7 +198,7 @@ Section LWEquivTree.
       specialize (Htmvalid msreset z Hmsreset_inp Heqz).
       specialize (Htmc_valid ms z' Hms_inp Heqz').
       apply tree_pop_reg.
-      rewrite noi_nonzero_succprec with (x := plus). 2: now apply noi_eqb_neq.
+      rewrite noi_nonzero_succprec with (x := delta). 2: now apply noi_eqb_neq.
       eapply tree_quant_minzero_pluspos.
       * symmetry. apply Hgroupsvalid.
       * rewrite ms_suffix_current_str with (ms := ms). 2: assumption.
@@ -197,18 +210,18 @@ Section LWEquivTree.
   (* Main theorem for repeated matching *)
   Lemma tRepeatMatcher'_valid:
     (* for all repeat matcher parameters, *)
-    forall rer greedy parenIndex parenCount mini plus,
+    forall rer greedy parenIndex parenCount mini delta,
       (* for any TMatcher tm that is valid with respect to some Linden regex lreg and direction dir, *)
     forall (tm: TMatcher) (lreg: regex) (dir: Direction),
       tm_valid tm rer lreg dir ->
       (* such that the defined groups of lreg correspond to the capture reset parameters of the repeat matcher, *)
       def_groups lreg = List.seq (parenIndex + 1) parenCount ->
       (* the corresponding tree repeat matcher recognizes lreg quantified accordingly to the parameters (for any fuel, provided the matcher does not run out of fuel) with direction dir. *)
-      forall fuel, tm_valid (fun s tmc => tRepeatMatcher' tm dir mini (NoI.N mini + plus)%NoI greedy s tmc parenIndex parenCount fuel) rer (Regex.Quantified greedy mini plus lreg) dir.
+      forall fuel, tm_valid (fun s tmc => tRepeatMatcher' tm dir mini (NoI.N mini + delta)%NoI greedy s tmc parenIndex parenCount fuel) rer (Regex.Quantified greedy mini delta lreg) dir.
   Proof.
-    intros rer greedy parenIndex parenCount mini plus tm lreg dir Htmvalid Hgroupsvalid fuel.
+    intros rer greedy parenIndex parenCount mini delta tm lreg dir Htmvalid Hgroupsvalid fuel.
     destruct mini as [|mini'].
-    - replace (NoI.N 0 + plus)%NoI with plus by now destruct plus. now apply tRepeatMatcher'_minzero_valid.
+    - replace (NoI.N 0 + delta)%NoI with delta by now destruct delta. now apply tRepeatMatcher'_minzero_valid.
     - apply tRepeatMatcher'_minnonzero_valid; auto. intro fuel0. now apply tRepeatMatcher'_minzero_valid.
   Qed.
 
