WarblreEquiv/GroupMapMS.v
@@ -41,4 +41,8 @@ Section GroupMapMS.
       GroupMap.find gid gm = Some (GroupMap.Range idx None) <->
       In (gid, idx) gl.
 
+  (* Disjointness of open groups list with list of defined groups; needed for capture reset case *)
+  Definition open_groups_disjoint (gl: open_groups) (def_groups: list group_id) :=
+    forall gid idx, In (gid, idx) gl -> ~In gid def_groups.
+
 End GroupMapMS.
